Changes to name abstraction

theories/NameAbstraction.v
@@ -1,31 +1,145 @@
 From Coq Require Import Classes.RelationClasses.
-From Nominal Require Import Alpha.
+From Nominal Require Export Nominal Fresh.
 From Nominal.Instances Require Import Name Prod Perm.
 
-#[universes(template=no)]
-Record NameAbstraction `{Nominal X} := mkAbstraction { abs :> (Name * X) }.
+#[universes(template=no),projections(primitive=yes)]
+Record NameAbstraction `{Nominal X} := mkAbstraction { name: Name; term: X }.
 Arguments NameAbstraction _ {_ _ _ _}.
 Arguments mkAbstraction {_ _ _ _ _} _.
 Notation " '[𝔸]' X " := (NameAbstraction X) (at level 1, no associativity, format "[𝔸] X").
-Notation " [ a ] x " := ({| abs := (a,x) |}) (at level 1, no associativity, format "[ a ] x").
+Notation " ⟦ a ⟧ x " := ({| name := a; term := x |}) (at level 1, no associativity, format "⟦ a ⟧ x").
 
 #[export] Instance name_abstraction_action `{Nominal X}: PermAction [𝔸]X := 
-    λ p a, mkAbstraction (p • (fst a), p • (snd a)). 
+    λ p abs, mkAbstraction (p • abs.(name)) (p • abs.(term)). 
 
 #[export] Instance name_abstraction_support `{Nominal X}: Support [𝔸]X := 
-    fun ax => let (a,x) := abs ax in (support x) ∖ {[a]}.
-    
+    fun abs => (support abs.(term)) ∖ {[abs.(name)]}.
+
+(* Old Alpha.v *)
+
+#[export] Instance alpha_equiv_e `{Nominal X}: Equiv [𝔸]X | 0 :=
+    λ x y, ∃ (c: Name), c #[x.(name), y.(name), x.(term), y.(term)] ∧ ⟨c,x.(name)⟩•x.(term) ≡@{X} ⟨c,y.(name)⟩•y.(term).
+
+#[export] Instance alpha_equiv_a `{Nominal X}: Equiv [𝔸]X | 1 := 
+    λ x y, ∀ (c: Name), c #[x.(name), y.(name), x.(term), y.(term)] → ⟨c,x.(name)⟩•x.(term) ≡@{X} ⟨c,y.(name)⟩•y.(term).
+
+Infix "≈α" := (alpha_equiv_e) (at level 70, no associativity).
+Infix "≈αₐ" := (alpha_equiv_a) (at level 70, no associativity).
+Notation "(≈α)" := (alpha_equiv_e) (only parsing).
+Notation "(≈αₐ)" := (alpha_equiv_a) (only parsing).
+
+(* Alpha relation analogue to freshness some/any *)
+Lemma alpha_some_any `{Nominal X} (a b: Name) (x y: X): ⟦a⟧x ≈α ⟦b⟧y ↔ ⟦a⟧x ≈αₐ ⟦b⟧y.
+Proof.
+    split; intros Ha. unfold alpha_equiv_e, alpha_equiv_a in *; simpl in *.
+    - intros; simpl in *; destruct Ha as [w [? Ha]]; destruct_and!;
+        rewrite (perm_expand _ w a), (perm_expand _ w b), <-!gact_compat, 
+            (fresh_fixpoint _ _ x), (fresh_fixpoint _ _ y), Ha;
+        try (apply not_eq_sym, name_neq_fresh_iff); auto.
+    - new c fresh a b x y; fresh_tac; exists c; split; [| apply Ha]; fresh_tac; intuition.
+Qed.
+
+(* Alpha relation is an equivalence. *)
+#[export] Instance alpha_equivalence_e `{Nominal X}: Equivalence (@alpha_equiv_e X _ _ _ _).
+Proof.
+    split.
+    - intros [a x]; destruct (exist_fresh (support a ∪ support x)) as [y []%not_elem_of_union];
+        exists y; split_and!; simpl; try (apply support_fresh); auto.
+    - intros [? ?] [? ?] [z ?]; exists z; intuition. 
+    - intros [a x] [b y] [c z] A A'; simpl in *;
+        new f fresh a x b y c z; fresh_tac; apply alpha_some_any in A,A'; exists f; split; simpl;
+            [| rewrite (A f), (A' f)]; intuition. 
+Qed.
+
+#[export] Instance alpha_equivalence_a `{Nominal X}: Equivalence (@alpha_equiv_a X _ _ _ _).
+Proof.
+    split.
+    - intros [] ? ?; simpl; reflexivity.
+    - intros [] [] HH b ?; specialize (HH b); intuition.
+    - intros [] [q p] [] H1 H2; apply alpha_some_any in H1,H2; apply alpha_some_any.
+        (* for some reason Coq cant find an instance for Transitive alpha_equiv_e, even though its
+           define just above. *)
+        pose proof (@Equivalence_Transitive _ _ alpha_equivalence_e).
+        transitivity ⟦q⟧p; auto.
+Qed.
+
+Lemma alpha_rename `{Nominal X} (a b: Name) (x: X): b#x → ⟦a⟧x ≈α ⟦b⟧(⟨a,b⟩•x).
+Proof.
+    intros; destruct (decide (a = b)); subst.
+    - apply alpha_some_any; repeat intro; simpl in *; rewrite perm_action_equal; reflexivity.
+    - new c fresh a b x (⟨a,b⟩ • x); fresh_tac; exists c; simpl; split; [intuition |]; 
+        rewrite (perm_expand _ b _), <-2!gact_compat, (fresh_fixpoint c b x), (swap_perm b a); auto.
+        apply not_eq_sym,name_neq_fresh_iff; auto.
+Qed.
+
+Lemma alpha_rename_swap `{Nominal X} (a b: Name) (x: X): b#x → ⟦a⟧x ≈α ⟦b⟧(⟨b,a⟩•x).
+Proof.
+    intros; destruct (decide (a = b)); subst.
+    - apply alpha_some_any; repeat intro; simpl in *; rewrite perm_action_equal; reflexivity.
+    - new c fresh a b x (⟨b,a⟩ • x); fresh_tac; exists c; simpl; split; [intuition |]; 
+        rewrite (perm_expand _ b _), <-2!gact_compat, (fresh_fixpoint c b x), (swap_perm b a); auto.
+        apply not_eq_sym,name_neq_fresh_iff; auto.
+Qed.
+
+(* Alpha relation properties *)
+Lemma alpha_inv_left `{Nominal X} (a b: Name) (x y: X): 
+    ⟦a⟧x ≈α ⟦b⟧y → ((a = b ∧ x ≡ y) ∨ (a #(b,y) ∧ x ≡ ⟨a,b⟩•y)).
+Proof.
+    destruct (decide (a = b)); subst; intros [w [wFr wFx]].
+    - left; split; [reflexivity |]; eapply perm_inj; intuition; eassumption.
+    - right; cut (a # b ∧ a # y); [intros [] |].
+        + split; [apply fresh_prod_iff; intuition |].
+            rewrite (perm_expand _ w _), <-!gact_compat, (fresh_fixpoint a w y), <-wFx, swap_perm; intuition; subst.
+            * symmetry; apply perm_action_duplicate.
+            * eapply name_fresh_false; eauto. 
+        + split; [apply name_neq_fresh_iff; assumption |].
+          cut (⟨w,b⟩ • ⟨w,b⟩ • y ≡ y); [intros HH1 | apply perm_action_duplicate].
+          cut (⟨w,b⟩ • ⟨w,a⟩ • w = a); [intros HH2 | rewrite perm_swap_left, perm_swap_neither; auto; apply not_eq_sym, name_neq_fresh_iff; intuition].
+          rewrite <-HH1,<-wFx; rewrite <-HH2 at 1; do 2 apply fresh_equivariant; intuition.
+Qed.
+
+Lemma alpha_inv_right `{Nominal X} (a b: Name) (x y: X): 
+    ((a = b ∧ x ≡ y) ∨ (a # (b,y) ∧ x ≡ ⟨a,b⟩•y)) → ⟦a⟧x ≈α ⟦b⟧y.
+Proof.
+    intros [[? HH] | [HH1%fresh_prod_iff HH2]]; new w fresh a b x y; fresh_tac; subst; exists w; simpl in *.
+    - split; [intuition |]; rewrite HH; reflexivity.
+    - split; [intuition |]; rewrite HH2, (perm_expand w a b), <-!gact_compat, (fresh_fixpoint w a y);
+        intuition; subst; eapply name_fresh_false; eauto.
+Qed.
+
+Lemma alpha_inv_iff `{Nominal X} (a b: Name) (x y: X): 
+    ⟦a⟧x ≈α ⟦b⟧y ↔ (a = b ∧ x ≡ y) ∨ (a # (b,y) ∧ x ≡ ⟨a,b⟩•y).
+Proof. split; [apply alpha_inv_left | apply alpha_inv_right]. Qed.
+
+Corollary alpha_inv_name_equiv_iff `{Nominal X} (a: Name) (x y: X): 
+    ⟦a⟧x ≈α ⟦a⟧y ↔ x ≡ y.
+Proof.
+    split; intros HH.
+    - apply alpha_inv_iff in HH as [? | [? H1]]; [| rewrite perm_action_equal in H1]; intuition.
+    - apply alpha_inv_iff; left; intuition.
+Qed.
+
+Lemma alpha_equivar `{Nominal X} (p: Perm) (a b: Name) (x y: X): 
+    ⟦a⟧x ≈α ⟦b⟧y → ⟦p•a⟧(p•x) ≈α ⟦p•b⟧(p•y).
+Proof.
+    intro HA; apply alpha_inv_iff; apply alpha_inv_iff in HA as [[? Hxy] | [Hby ?]].
+    - left; split; subst; [| rewrite Hxy]; auto.
+    - right; split.
+        + apply fresh_prod_iff in Hby as []; apply fresh_prod_iff; split; apply fresh_equivariant; auto.
+        + rewrite <-perm_swap_distr; apply perm_inj; assumption.
+Qed.
+
+(* Old Alpha.v *)
+
 (* Given X nominal, the pair (name * X) is a nominal type module (≈α) *)
 #[export] Instance name_abstraction_equiv `{Nominal X}: Equiv [𝔸]X := (≈α).
-#[export] Instance name_abstraction_equivalence `{Nominal X}: Equivalence (name_abstraction_equiv (X := X)).
+#[export] Instance name_abstraction_equivalence `{Nominal X}: Equivalence name_abstraction_equiv.
 Proof.
     split; unfold name_abstraction_equiv; repeat intro.
-    - destruct x as [[a x]]; simpl; new b fresh a x; fresh_tac; exists b; split; intuition.
-    - destruct x as [[a x]]; destruct y as [[b y]]; simpl in *; destruct H1 as [c []];
-        exists c; split; intuition.
-    - destruct x as [[a x]]; destruct y as [[b y]]; destruct z as [[c z]]; apply alpha_some_any in H1,H2;
-        simpl in *; new f fresh a b c x y z; fresh_tac; exists f; split; [intuition | etransitivity]; 
-        [eapply H1 | eapply H2]; intuition.
+    - new b fresh x.(name) x.(term); fresh_tac; exists b; split; auto.
+    - destruct H1 as [c []]; exists c; split; intuition.
+    - apply alpha_some_any in H1,H2. new f fresh x.(name) y.(name) z.(name) x.(term) y.(term) z.(term); fresh_tac;
+      exists f; split; [intuition | etransitivity]; [eapply H1 | eapply H2]; intuition.
 Qed.
 
 #[export] Instance name_abstraction_perm `{Nominal X}: PermT [𝔸]X.
@@ -33,26 +147,27 @@ Proof.
     Opaque alpha_equiv_e.
     split.
     - exact name_abstraction_equivalence.
-    - intros p q Heq1 [[a x]] [[b y]] Heq2.
+    - intros p q Heq1 x y Heq2.
         unfold action, name_abstraction_action, equiv, name_abstraction_equiv.
         unfold equiv, name_abstraction_equiv in Heq2; simpl in *.
-        new w fresh p q a b x y (p • x) (q • y); exists w; apply alpha_some_any in Heq2; split.
+        new w fresh p q x.(name) y.(name) x.(term) y.(term) (p•x.(term)) (q•y.(term));
+        exists w; apply alpha_some_any in Heq2; split.
         + split_and!; try apply name_fresh_action; split_union; apply support_fresh; auto.
         + cut ((p • w ≡ w) ∧ (q • w ≡ w)); [intros [W1 W2] | split; apply perm_notin_domain_id; auto].
-            (* slow *)rewrite <-W1 at 1; (* slow *)rewrite <-W2 at 2.
+            simpl in *; (* slow *)rewrite <-W1 at 1; (* slow *)rewrite <-W2 at 2.
             rewrite 2!gact_compat, <-2!perm_comm_distr, <-2!gact_compat, Heq1.
             apply perm_inj. unfold alpha_equiv_a in *; apply Heq2; split_and!; split_union;
             apply support_fresh; auto. split_union. split_union.
-    - intros [[a x]]; unfold action, name_abstraction_action, prod_action, equiv, name_abstraction_equiv; simpl.
-        apply alpha_some_any; intros w ?; rewrite 2!gact_id; reflexivity.
-    - intros ? ? [[a x]]; unfold action, name_abstraction_action, prod_action, equiv, name_abstraction_equiv;
+    - intros x; unfold action, name_abstraction_action, equiv, name_abstraction_equiv; simpl.
+        apply alpha_some_any; intros w ?; simpl; rewrite 2!gact_id; reflexivity.
+    - intros ? ? x; unfold action, name_abstraction_action, prod_action, equiv, name_abstraction_equiv; simpl.
         apply alpha_some_any; intros w ?; simpl in *; rewrite <-2!gact_compat; reflexivity.
 Qed.
 
 #[export] Instance name_abstraction_nominal `{Nominal X}: Nominal [𝔸]X.
 Proof. split.
     - exact name_abstraction_perm.
-    - intros [[a x]] b c ? ?; destruct (decide (b = c)), (decide (b = a)), (decide (c = a));
+    - intros x a b ? ?; destruct (decide (a = b)), (decide (a = x.(name))), (decide (b = x.(name)));
           try (subst; congruence || subst; apply perm_action_equal); unfold support, name_abstraction_support in *; simpl in *.
         + subst; apply not_elem_of_difference in H1 as []; apply not_elem_of_difference in H2 as [].   (* subst. apply support_fresh in H1. as [?%name_neq_fresh_iff ?]. congruence. *)
           * unfold action,equiv,name_abstraction_equiv,name_abstraction_action ; simpl.
@@ -72,139 +187,112 @@ Proof. split.
             symmetry; apply alpha_rename_swap, support_fresh; auto.
           * set_solver.
           * set_solver. 
-        + new z fresh (⟨b,c⟩ • a) a (⟨b,c⟩ • x) x; fresh_tac; exists z; simpl; split; simpl; [intuition |].
-          rewrite perm_swap_neither, (fresh_fixpoint b c x); auto.
+        + new z fresh (⟨a,b⟩ • x.(name)) x.(name) (⟨a,b⟩ • x.(term)) x.(term); fresh_tac; exists z; simpl; repeat (split; auto).
+          rewrite perm_swap_neither, (fresh_fixpoint a b x.(term)); auto.
           * apply not_elem_of_difference in H1 as []; apply support_fresh; auto; set_solver.
           * apply not_elem_of_difference in H2 as []; apply support_fresh; auto; set_solver.
 Qed.
 
 (* Basic properties *)
 Lemma name_abstraction_rename `{Nominal X} (a b: Name) (x: X): 
-    b#x → [a]x ≡ [b](⟨a,b⟩ • x).
+    b#x → ⟦a⟧x ≡ ⟦b⟧(⟨a,b⟩•x).
 Proof. apply alpha_rename. Qed.
 
 Lemma name_abstraction_rename_swap `{Nominal X} (a b: Name) (x: X): 
-    b#x → [a]x ≡ [b](⟨b,a⟩ • x).
+    b#x → ⟦a⟧x ≡ ⟦b⟧(⟨b,a⟩•x).
 Proof. apply alpha_rename_swap. Qed.
 
-Lemma nabs_action `{Nominal X} p a (x: X): p • [a]x = [p • a](p • x).
+Lemma nabs_action `{Nominal X} p a (x: X): p•(⟦a⟧x) = ⟦p•a⟧(p•x).
 Proof. auto. Qed.
 
-Lemma nabs_support `{Nominal X} a (x: X): support [a]x = support x ∖ {[a]}.
+Lemma nabs_support `{Nominal X} a (x: X): support ⟦a⟧x = support x ∖ {[a]}.
 Proof. auto. Qed.
 
-Lemma nabs_inv `{Nominal X} a (x x': X): [a]x ≡ [a]x' ↔ x ≡ x'.
+Lemma nabs_inv `{Nominal X} a (x x': X): ⟦a⟧x ≡ ⟦a⟧x' ↔ x ≡ x'.
 Proof. split; intros HH.
     - unfold equiv, name_abstraction_equiv in HH; apply alpha_inv_name_equiv_iff in HH; auto. 
     - apply (alpha_inv_name_equiv_iff a) in HH; assumption.
 Qed.
 
-Lemma fresh_same_alpha_class `{Nominal X} a (x: X): a # [a]x.
+Lemma fresh_same_nabs `{Nominal X} a (x: X): a # ⟦a⟧x.
 Proof.
     destruct (exist_fresh (support x ∖ {[a]})) as [w ?]; exists w.
     split; [auto |].
     apply not_elem_of_difference in H1 as [].
     + unfold equiv, name_abstraction_equiv; simpl.
-      rewrite name_action_left; pose proof (@Equivalence_Symmetric _ _ alpha_equivalence_e) as S;
+      rewrite nabs_action, name_action_left; pose proof (@Equivalence_Symmetric _ _ alpha_equivalence_e) as S;
       symmetry; apply alpha_rename, support_fresh; assumption.
     + apply elem_of_singleton in H1; subst; apply perm_action_equal.
 Qed.
 
-Lemma alpha_class_inv1 `{Nominal X} (a a': Name) (x: X): 
-    a = a' ∨ (a ≠ a' ∧ a' # x) → a' # [a]x.
+Lemma fresh_nabs_left `{Nominal X} (a a': Name) (x: X): 
+    a = a' ∨ (a ≠ a' ∧ a' # x) → a' # ⟦a⟧x.
 Proof.
-    intros [EqA | [? F]]; [rewrite EqA | destruct (decide (a = a')); subst]; try apply fresh_same_alpha_class.
-    destruct (exist_fresh (support a ∪ support a' ∪ support x)) as [w ?]; exists w.
+    intros [EqA | [? F]]; subst; [apply fresh_same_nabs |].
+    destruct (exist_fresh (support a ∪ support a' ∪ support x)) as [w ?]; exists w;
     split; [set_solver |].
     unfold equiv, name_abstraction_equiv; simpl.
-    rewrite perm_swap_neither; try set_solver.
-    apply alpha_inv_name_equiv_iff, fresh_fixpoint; [assumption | apply support_fresh]; set_solver.
+    rewrite nabs_action,perm_swap_neither; try set_solver.
+    apply alpha_inv_name_equiv_iff, fresh_fixpoint;
+    [assumption | apply support_fresh]; set_solver.
 Qed.
 
-Lemma alpha_class_inv2 `{Nominal X} (a a': Name) (x: X): 
-    a' # [a]x → a = a' ∨ (a ≠ a' ∧ a' # x).
+Lemma fresh_nabs_right `{Nominal X} (a a': Name) (x: X): 
+    a' # ⟦a⟧x → a = a' ∨ (a ≠ a' ∧ a' # x).
 Proof.
     intros F; destruct (decide (a = a')); subst; [intuition |].
     right. (* a ≠ a' *) split; auto.
-    destruct (exist_fresh (support a ∪ support a' ∪ support x ∪ support [a]x)) as [w ?]; exists w.
-    split; [set_solver |]; apply some_any_iff in F; cut (w ∉ support [a]x); [intros Hw | set_solver].
-    specialize (F w Hw); unfold equiv, name_abstraction_equiv in F. 
+    destruct (exist_fresh (support a ∪ support a' ∪ support x ∪ support ⟦a⟧x)) as [w ?]; exists w.
+    split; [set_solver |]; apply some_any_iff in F; cut (w ∉ support ⟦a⟧x); [intros Hw | set_solver].
+    specialize (F w Hw); unfold equiv, name_abstraction_equiv in F; rewrite nabs_action in F. 
     simpl in F. assert (L: ⟨a',w⟩ • a = a). { apply perm_swap_neither; set_solver. }
     rewrite L in F; apply alpha_inv_name_equiv_iff in F; assumption.
 Qed.
 
-Lemma alpha_class_inv `{Nominal X} (a a': Name) (x: X): 
-    a = a' ∨ (a ≠ a' ∧ a' # x) ↔ a' # [a]x.
-Proof. split; [apply alpha_class_inv1 | apply alpha_class_inv2]. Qed.
+Lemma fresh_nabs `{Nominal X} (a a': Name) (x: X): 
+    a = a' ∨ (a ≠ a' ∧ a' # x) ↔ a' # ⟦a⟧x.
+Proof. split; [apply fresh_nabs_left | apply fresh_nabs_right]. Qed.
+
+#[global] Instance name_abstraction_proper `{Nominal X}: 
+    Proper (equiv ==> equiv ==> (@name_abstraction_equiv X _ _ _ _)) mkAbstraction.
+Proof. repeat intro; unfold name_abstraction_equiv; simpl; rewrite H1; apply alpha_inv_name_equiv_iff; assumption. Qed.
+
 
 #[global] Instance name_abstraction_rw1 `{Nominal X}: 
-    ∀a, Proper (equiv ==> alpha_equiv_e) (pair a).
-Proof. repeat intro; apply alpha_inv_iff; left; tauto. Qed.
+    ∀ a, Proper (equiv ==> (@name_abstraction_equiv X _ _ _ _)) (mkAbstraction a).
+Proof. repeat intro. unfold name_abstraction_equiv; apply alpha_inv_name_equiv_iff; auto. Qed.
 
 #[global] Instance name_abstraction_rw2 `{Nominal X}: 
-    Proper (alpha_equiv_e ==> (@name_abstraction_equiv X _ _ _ _)) mkAbstraction.
-Proof. repeat intro; unfold name_abstraction_equiv; simpl; assumption. Qed.
-
-#[global] Instance name_abstraction_rw3 `{Nominal X}: 
     Proper ((@name_abstraction_equiv X _ _ _ _) ==> (@name_abstraction_equiv X _ _ _ _) ==> flip impl) equiv.
 Proof.
-    repeat intro; unfold name_abstraction_equiv in *; 
-    destruct x as [[a x]]; destruct y as [[a' x']];
-    destruct x0 as [[b z]]; destruct y0 as [[b' z']]; simpl; unfold equiv in *.
-    (* for some reason Coq cant find an instance for Transitive or Symmetric alpha_equiv_e *)
+    repeat intro. unfold name_abstraction_equiv in *.
     pose proof (@Equivalence_Transitive _ _ alpha_equivalence_e) as T.
     pose proof (@Equivalence_Symmetric _ _ alpha_equivalence_e) as S.
-    apply T with [a']x'; auto; apply T with [b']z'; auto.
+    apply T with ⟦y.(name)⟧y.(term); auto; apply T with ⟦y0.(name)⟧y0.(term); auto.
 Qed.
 
-#[global] Instance name_abstraction_rw4 `{Nominal X}: 
-    ∀ a (x : X), ProperProxy ((@name_abstraction_equiv X _ _ _ _)) [a]x.
+#[global] Instance name_abstraction_rw3 `{Nominal X}: 
+    ∀ a (x : X), ProperProxy (@name_abstraction_equiv X _ _ _ _) ⟦a⟧x.
 Proof. 
     unfold ProperProxy,name_abstraction_equiv; repeat intro.
     pose proof (@Equivalence_Reflexive _ _ alpha_equivalence_e) as F.
     auto.
 Qed.
 
-Lemma name_abstraction_inv `{Nominal} (a b: Name) (x y: X):
-    [a]x ≡ [b]y ↔ (a = b ∧ x ≡ y) ∨ ((a # [b]y) ∧ x ≡ ⟨a,b⟩ • y).
+Lemma name_abstraction_inv `{Nominal X} (a b: Name) (x y: X):
+    ⟦a⟧x ≡ ⟦b⟧y ↔ (a = b ∧ x ≡ y) ∨ ((a # ⟦b⟧y) ∧ x ≡ ⟨a,b⟩•y).
 Proof.
     split; intro HH.
     - apply alpha_inv_iff in HH as [? | [HHH ?]].
         + left; assumption.
-        + right; split; try tauto; apply alpha_class_inv; right; apply fresh_prod_iff in HHH as []; split.
+        + right; split; try tauto; apply fresh_nabs; right; apply fresh_prod_iff in HHH as []; split.
             * apply not_eq_sym, name_neq_fresh_iff; assumption.
             * assumption. 
     - destruct HH as [[] | [HH1 HH2]].
         + subst; rewrite H2; reflexivity.
-        + apply alpha_class_inv in HH1 as []; subst.
+        + apply fresh_nabs in HH1 as []; subst.
             * apply nabs_inv; rewrite HH2; apply perm_action_equal.
             * apply alpha_inv_iff; right; split.
                 -- apply fresh_prod_iff; split; [apply name_fresh_iff,name_neq_fresh_iff |]; tauto.
                 -- assumption.
 Qed.
-
-(* Concretion *)
-Section Concretion.
-    Context `{Nominal X}.
-
-    Definition concretion (F: [𝔸]X) (b: Name): option X :=
-       let (a,x) := abs F in
-       if (decide (a = b)) then Some x else
-       if (decide (b ∉ support x)) then Some (⟨a,b⟩ • x)
-       else None.
-    
-    Lemma concretion_eq a b (x: X): 
-        a = b → concretion ([a]x) b ≡ Some x.
-    Proof. 
-        intros; subst; unfold concretion; simpl; destruct (decide _); subst;
-        [reflexivity | congruence].
-    Qed.
-
-    Lemma concretion_notin a b (x: X): 
-        a ≠ b → b ∉ support x → concretion ([a]x) b ≡ Some (⟨a,b⟩ • x).
-    Proof. 
-        intros; subst; unfold concretion; simpl; destruct (decide _); subst;
-        [congruence | destruct (decide _); [reflexivity | set_solver]]. 
-    Qed.
-    
-End Concretion.
