theories/Concretion.v
@@ -1,0 +1,26 @@
+From Nominal Require Import Nominal NameAbstraction.
+
+Section Concretion.
+    Context `{Nominal X}.
+
+    Definition concretion (F: [𝔸]X) (b: Name): option X :=
+       let (a,x) := abs F in
+       if (decide (a = b)) then Some x else
+       if (decide (b ∉ support x)) then Some (⟨a,b⟩ • x)
+       else None.
+    
+    Lemma concretion_eq a b (x: X): 
+        a = b → concretion ([a]x) b ≡ Some x.
+    Proof. 
+        intros; subst; unfold concretion; simpl; destruct (decide _); subst;
+        [reflexivity | congruence].
+    Qed.
+
+    Lemma concretion_notin a b (x: X): 
+        a ≠ b → b ∉ support x → concretion ([a]x) b ≡ Some (⟨a,b⟩ • x).
+    Proof. 
+        intros; subst; unfold concretion; simpl; destruct (decide _); subst;
+        [congruence | destruct (decide _); [reflexivity | set_solver]]. 
+    Qed.
+    
+End Concretion.
